src/lowparse/LowParse.Low.Combinators.fst
@@ -7,7 +7,7 @@ module U32 = FStar.UInt32
 module HS = FStar.HyperStack
 module HST = FStar.HyperStack.ST
 
-#reset-options "--z3rlimit 128 --max_fuel 32 --max_ifuel 32 --z3cliopt smt.arith.nl=false"
+#reset-options "--z3rlimit 256 --max_fuel 32 --max_ifuel 32 --z3cliopt smt.arith.nl=false"
 
 inline_for_extraction
 let validate32_nondep_then
@@ -21,14 +21,13 @@ let validate32_nondep_then
   (p2' : validator32 p2)
 : Tot (validator32 (nondep_then p1 p2))
 = fun (input: pointer buffer8) (len: pointer U32.t) ->
-  let h = HST.get () in
   if p1' input len
   then begin
-    let h1 = HST.get () in
     let res = p2' input len in
-    let h' = HST.get () in
     res
   end else false
+
+#reset-options "--z3rlimit 128 --max_fuel 32 --max_ifuel 32 --z3cliopt smt.arith.nl=false"
 
 inline_for_extraction
 let validate_nochk32_nondep_then
@@ -110,56 +109,7 @@ let validate_nochk32_constant_size
 = fun (input: pointer buffer8) (len: pointer U32.t) ->
   advance_slice_ptr input len sz
 
-inline_for_extraction
-val validate_nochk_truncate32
-  (#k: parser_kind)
-  (#t: Type0)
-  (p: parser k t)
-  (v: validator_nochk32 p)
-  (input: pointer buffer8)
-  (sz: pointer U32.t)
-: HST.Stack unit
-  (requires (fun h ->
-    is_slice_ptr h input sz /\
-    Some? (parse p (B.as_seq h (B.get h input 0)))
-  ))
-  (ensures (fun h _ h' ->
-    B.modifies_2 input sz h h' /\
-    is_slice_ptr h' input sz /\ (
-    let sq = B.as_seq h (B.get h input 0) in
-    let (Some (res, consumed)) = parse p sq in
-    U32.v (B.get h' sz 0) == consumed /\
-    B.get h' input 0 == B.sub (B.get h input 0) 0ul (U32.uint_to_t consumed) /\ (
-    let sq' = B.as_seq h' (B.get h' input 0) in
-    sq' == Seq.slice sq 0 consumed /\ (
-    let psq' = parse p sq' in
-    Some? psq' /\ (
-    let (Some (res', consumed')) = psq' in
-    res == res' /\
-    (consumed' <: nat) == (consumed <: nat)
-  ))))))
-
-let validate_nochk_truncate32 #k #t p v input sz =
-  let h = HST.get () in
-  let input0 = B.index input 0ul in
-  let sz0 = B.index sz 0ul in
-  v input sz ;
-  let sz1 = B.index sz 0ul in
-  let len' = U32.sub sz0 sz1 in
-  let input' = B.sub input0 0ul len' in
-  B.upd input 0ul input';
-  B.upd sz 0ul len';
-  let h' = HST.get () in
-  let f () : Lemma (
-    let (Some (res, consumed)) = parse p (B.as_seq h (B.get h input 0)) in
-    let ps' = parse p (B.as_seq h' (B.get h' input 0)) in
-    Some? ps' /\ (
-    let (Some (res', consumed')) = ps' in
-    res == res' /\ (consumed <: nat) == (consumed' <: nat)
-  )) =
-    assert (no_lookahead_weak_on p (B.as_seq h (B.get h input 0)) (B.as_seq h' (B.get h' input 0)))
-  in
-  f ()
+module M = FStar.Modifies
 
 inline_for_extraction
 val nondep_then_fst
@@ -175,23 +125,17 @@ val nondep_then_fst
 : HST.Stack unit
   (requires (fun h ->
     is_slice_ptr h input sz /\
-    Some? (parse (p1 `nondep_then` p2) (B.as_seq h (B.get h input 0)))
+    Some? (parse_from_slice_ptr (nondep_then p1 p2) h input sz)
   ))
   (ensures (fun h _ h' ->
-    B.modifies_2 input sz h h' /\
-    is_slice_ptr h' input sz /\ (
-    let (Some (res1, consumed1)) = parse p1 (B.as_seq h (B.get h input 0)) in
-    U32.v (B.get h' sz 0) == consumed1 /\
-    B.get h' input 0 == B.sub (B.get h input 0) 0ul (U32.uint_to_t consumed1) /\ (
-    let ps1' = parse p1 (B.as_seq h' (B.get h' input 0)) in
-    Some? ps1' /\ (
-    let (Some (res1', consumed1')) = parse p1 (B.as_seq h' (B.get h' input 0)) in
-    res1 == res1' /\
-    (consumed1 <: nat) == (consumed1' <: nat)
-  )))))
+    M.modifies (loc_slice input sz) h h' /\
+    includes_slice_ptr h h' input sz /\ (
+    let (Some ((x, _), _)) = parse_from_slice_ptr (nondep_then p1 p2) h input sz in
+    exactly_parse_from_slice_ptr p1 h' input sz == Some x
+  )))
 
 let nondep_then_fst #k1 #t1 #p1 p1' #k2 #t2 p2 input sz =
-  validate_nochk_truncate32 p1 p1' input sz
+  truncate32 p1' input sz
 
 inline_for_extraction
 val nondep_then_snd
@@ -208,26 +152,18 @@ val nondep_then_snd
 : HST.Stack unit
   (requires (fun h ->
     is_slice_ptr h input sz /\
-    Some? (parse (p1 `nondep_then` p2) (B.as_seq h (B.get h input 0)))
+    Some? (parse_from_slice_ptr (nondep_then p1 p2) h input sz)
   ))
   (ensures (fun h _ h' ->
-    B.modifies_2 input sz h h' /\
-    is_slice_ptr h' input sz /\ (
-    let sq = B.as_seq h (B.get h input 0) in
-    let (Some (_, consumed1)) = parse p1 sq in
-    let (Some (res2, consumed2)) = parse p2 (Seq.slice sq consumed1 (Seq.length sq)) in
-    U32.v (B.get h' sz 0) == consumed2 /\
-    B.get h' input 0 == B.sub (B.get h input 0) (U32.uint_to_t consumed1) (U32.uint_to_t consumed2) /\ (
-    let ps2' = parse p2 (B.as_seq h' (B.get h' input 0)) in
-    Some? ps2' /\ (
-    let (Some (res2', consumed2')) = parse p2 (B.as_seq h' (B.get h' input 0)) in
-    res2 == res2' /\
-    (consumed2 <: nat) == (consumed2' <: nat)
-  )))))
+    M.modifies (loc_slice input sz) h h' /\
+    includes_slice_ptr h h' input sz /\ (
+    let (Some ((_, x), _)) = parse_from_slice_ptr (nondep_then p1 p2) h input sz in
+    exactly_parse_from_slice_ptr p2 h' input sz == Some x
+  )))
 
 let nondep_then_snd #k1 #t1 #p1 p1' #k2 #t2 #p2 p2' input sz =
   p1' input sz;
-  validate_nochk_truncate32 p2 p2' input sz
+  truncate32 p2' input sz
 
 inline_for_extraction
 let make_total_constant_size_parser32
